Begin L3-L4 translation

theories/L4_CPS/L3_to_L4.v
@@ -3,15 +3,57 @@
     mutually recursive functions, data constructors, and pattern matching.
 *)
 Require Import Arith BinNat String List Omega Program Psatz.
+Require Export Common.Common.  (* shared namespace *)
 Open Scope N_scope.
 Opaque N.add.
 Opaque N.sub.
 
-Require L3.term.
+Require Import L3.program.
 
-Require Import simpleCPS.
+Require L3.
+Module L3eval := L3.wndEval.
+Module L3 := L3.term.
+Require Import  simpleCPS.
 
+Definition dcon_of_con (i : inductive) (n : nat) := N.of_nat n.
 
+Fixpoint translate (t : L3.Term) : simpleCPS.exp :=
+  match t with
+  | L3.TRel n => Var_e (N.of_nat n)
+  | L3.TSort s => Var_e 0 (* encode with TConst ? *)
+  | L3.TProd n t => Var_e 0  (* same ? *)
+  | L3.TLambda n t => Lam_e (translate t)
+  | L3.TLetIn n t u => Let_e (translate t) (translate u)
+  | L3.TApp t u => App_e (translate t) (translate u)
+  | L3.TConst s => Var_e 0 (* FIXME *)
+  | L3.TInd i => Var_e 0 (* FIXME *)
+  | L3.TConstruct ind c args =>
+    let fix args' l :=
+        match l with
+        | L3.tnil => nil
+        | L3.tcons t ts => cons (translate t) (args' ts)
+        end
+    in Con_e (dcon_of_con ind c) (args' args)
+  | L3.TCase n t brs =>
+    let fix brs' n l :=
+      match l with
+      | L3.tnil => nil
+      | L3.tcons t ts => cons (n, 0 (* FIXME *), translate t) (brs' (n + 1)%N ts)
+      end
+    in Match_e (translate t) (brs' (0%N) brs)
+  | L3.TFix d n =>
+    let fix defs' l :=
+        match l with
+        | L3.dnil => nil
+        | L3.dcons na t k l' => cons (translate t) (defs' l')
+        end
+    in Proj_e (Fix_e (defs' d)) (N.of_nat n)
+  end.
 
+Theorem translate_correct (e : environ) (t t' : L3.Term) :
+  L3eval.wndEval e t t' -> (* small step non-deterministic *)
+  eval (translate t) (translate t') (* big-step deterministic *).
+Proof.
+  induction 1. simpl. red in H. 
 
 
